Weidenbach_Book/Watched_Literals_Watch_List_Domain_Enumeration.thy
@@ -1,5 +1,5 @@
 theory Watched_Literals_Watch_List_Domain_Enumeration
-  imports Watched_Literals_Watch_List_Enumeration Watched_Literals_Watch_List_Domain
+  imports Watched_Literals_Watch_List_Enumeration Watched_Literals.Watched_Literals_Watch_List_Domain
 begin
 
 context isasat_input_ops
@@ -35,7 +35,7 @@ lemma find_decomp_target_wl_D_find_decomp_target_wl:
   shows
     \<open>find_decomp_target_wl a S \<le> \<Down>(find_decomp_target_wl_D_ref S) (find_decomp_target_wl a' S')\<close>
   using assms unfolding find_decomp_target_wl_def
-  by (cases S') (auto intro!: RES_refine)
+  by (cases S') (auto intro!: RES_refine simp: literals_are_\<L>\<^sub>i\<^sub>n_def blits_in_\<L>\<^sub>i\<^sub>n_def)
 
 lemma is_\<L>\<^sub>a\<^sub>l\<^sub>l_add_mset_already_in:
   \<open>x \<in># N \<Longrightarrow> is_\<L>\<^sub>a\<^sub>l\<^sub>l (add_mset x N) \<longleftrightarrow>  is_\<L>\<^sub>a\<^sub>l\<^sub>l N\<close>
@@ -52,7 +52,7 @@ lemma negate_mode_bj_unit_wl_D_negate_mode_bj_unit_wl:
   using assms
   apply (refine_vcg find_decomp_target_wl_D_find_decomp_target_wl)
   apply (auto simp: mset_take_mset_drop_mset' uminus_\<A>\<^sub>i\<^sub>n_iff all_lits_of_mm_add_mset
-     all_lits_of_m_add_mset in_all_lits_of_mm_uminus_iff
+     all_lits_of_m_add_mset in_all_lits_of_mm_uminus_iff literals_are_\<L>\<^sub>i\<^sub>n_def blits_in_\<L>\<^sub>i\<^sub>n_def
       intro!: is_\<L>\<^sub>a\<^sub>l\<^sub>l_add_mset_already_in[THEN iffD2] dest:(* in_all_lits_of_mm_uminusD *))
   using is_\<L>\<^sub>a\<^sub>l\<^sub>l_def by blast
 
@@ -66,7 +66,7 @@ definition negate_mode_bj_nonunit_wl_D
     ASSERT(negate_mode_bj_nonunit_wl_D_inv S);
     let C = DECO_clause_l (get_trail_wl S);
     (S, K) \<leftarrow> find_decomp_target_wl (count_decided (get_trail_wl S)) S;
-    i \<leftarrow> get_fresh_index (get_clauses_wl S);
+    i \<leftarrow> get_fresh_index_wl (get_clauses_wl S) (get_unit_clauses_wl S) (get_watched_wl S);
     propagate_nonunit_and_add_wl K C i S
   })\<close>
 
@@ -74,6 +74,77 @@ lemma is_\<L>\<^sub>a\<^sub>l\<^sub>l_add_all_lits_of_m:
   \<open>is_\<L>\<^sub>a\<^sub>l\<^sub>l (all_lits_of_mm B) \<Longrightarrow> atms_of A \<subseteq> atms_of_mm B \<Longrightarrow> is_\<L>\<^sub>a\<^sub>l\<^sub>l (all_lits_of_m A + all_lits_of_mm B)\<close>
   unfolding is_\<L>\<^sub>a\<^sub>l\<^sub>l_def
   by (auto simp: in_all_lits_of_m_ain_atms_of_iff in_all_lits_of_mm_ain_atms_of_iff)
+
+lemma literals_are_\<L>\<^sub>i\<^sub>n_propagate_nonunit_and_add_wl:
+  assumes
+    lits: \<open>literals_are_\<L>\<^sub>i\<^sub>n T'\<close> and
+    le: \<open>2 \<le> count_decided (get_trail_wl S')\<close> and
+    i': \<open>i' \<notin># dom_m (get_clauses_wl T')\<close> and
+    atms: \<open>atms_of (DECO_clause (get_trail_wl S'))
+     \<subseteq> atms_of_ms ((\<lambda>x. mset (fst x)) ` set_mset (ran_m (get_clauses_wl T'))) \<union>
+        atms_of_mm (get_unit_init_clss_wl T')\<close>
+  shows \<open>literals_are_\<L>\<^sub>i\<^sub>n
+          (M',
+           fmupd i' (DECO_clause_l (get_trail_wl S'), b) (get_clauses_wl T'), None,
+           get_unit_init_clss_wl T', get_unit_learned_clss_wl T', Q, (get_watched_wl T')
+           (DECO_clause_l (get_trail_wl S') ! 0 :=
+              get_watched_wl T' (DECO_clause_l (get_trail_wl S') ! 0) @
+              [(i', DECO_clause_l (get_trail_wl S') ! Suc 0)],
+          DECO_clause_l (get_trail_wl S') ! Suc 0 :=
+            get_watched_wl T' (DECO_clause_l (get_trail_wl S') ! Suc 0) @
+            [(i', DECO_clause_l (get_trail_wl S') ! 0)]))\<close>
+  (is \<open>literals_are_\<L>\<^sub>i\<^sub>n ?S\<close>) and
+  \<open>DECO_clause_l (get_trail_wl S') ! 0 = DECO_clause_l (get_trail_wl S') ! Suc 0 \<Longrightarrow>
+    literals_are_\<L>\<^sub>i\<^sub>n
+     (M',
+      fmupd i' (DECO_clause_l (get_trail_wl S'), True) (get_clauses_wl T'), None, get_unit_init_clss_wl T',
+      get_unit_learned_clss_wl T', Q, (get_watched_wl T')
+      (DECO_clause_l (get_trail_wl S') ! 0 :=
+         get_watched_wl T' (DECO_clause_l (get_trail_wl S') ! 0) @
+         [(i', DECO_clause_l (get_trail_wl S') ! 0), (i', DECO_clause_l (get_trail_wl S') ! 0)]))\<close>
+  (is \<open>?eq \<Longrightarrow> literals_are_\<L>\<^sub>i\<^sub>n ?S'\<close>)
+proof -
+  have lall: \<open>is_\<L>\<^sub>a\<^sub>l\<^sub>l (all_lits_of_mm ((\<lambda>C. mset (fst C)) `# ran_m (get_clauses_wl T')
+        + get_unit_clauses_wl T'))\<close> and
+    blits: \<open>blits_in_\<L>\<^sub>i\<^sub>n T'\<close>
+    using lits unfolding literals_are_\<L>\<^sub>i\<^sub>n_def
+    by fast+
+  have \<open>is_\<L>\<^sub>a\<^sub>l\<^sub>l (all_lits_of_mm ((\<lambda>C. mset (fst C)) `# ran_m (get_clauses_wl ?S)
+        + get_unit_clauses_wl ?S))\<close>
+    using i' atms
+    by (auto simp: ran_m_mapsto_upd_notin all_lits_of_mm_add_mset
+        intro!: is_\<L>\<^sub>a\<^sub>l\<^sub>l_add_all_lits_of_m[unfolded get_unit_clauses_wl_alt_def]
+        lall[unfolded get_unit_clauses_wl_alt_def])
+  moreover have blits: \<open>blits_in_\<L>\<^sub>i\<^sub>n ?S\<close>
+    using blits  i' atms le lall unfolding length_DECO_clause_l[symmetric] is_\<L>\<^sub>a\<^sub>l\<^sub>l_def
+    by (cases \<open>DECO_clause_l (get_trail_wl S')\<close>; cases \<open>tl (DECO_clause_l (get_trail_wl S'))\<close>)
+      (auto simp: ran_m_mapsto_upd_notin all_lits_of_mm_add_mset blits_in_\<L>\<^sub>i\<^sub>n_def
+        in_\<L>\<^sub>a\<^sub>l\<^sub>l_atm_of_\<A>\<^sub>i\<^sub>n DECO_clause_l_DECO_clause[symmetric] Ball_def
+        in_all_lits_of_mm_ain_atms_of_iff all_conj_distrib
+        watched_by_alt_def get_unit_clauses_wl_alt_def
+        simp del: DECO_clause_l_DECO_clause)
+  ultimately show \<open>literals_are_\<L>\<^sub>i\<^sub>n ?S\<close>
+    unfolding literals_are_\<L>\<^sub>i\<^sub>n_def by blast
+
+
+  have \<open>is_\<L>\<^sub>a\<^sub>l\<^sub>l (all_lits_of_mm ((\<lambda>C. mset (fst C)) `# ran_m (get_clauses_wl ?S')
+        + get_unit_clauses_wl ?S'))\<close>
+    using i' atms
+    by (auto simp: ran_m_mapsto_upd_notin all_lits_of_mm_add_mset
+        intro!: is_\<L>\<^sub>a\<^sub>l\<^sub>l_add_all_lits_of_m[unfolded get_unit_clauses_wl_alt_def]
+        lall[unfolded get_unit_clauses_wl_alt_def])
+  moreover have blits: \<open>?eq \<Longrightarrow> blits_in_\<L>\<^sub>i\<^sub>n ?S'\<close>
+    using blits  i' atms le lall unfolding length_DECO_clause_l[symmetric] is_\<L>\<^sub>a\<^sub>l\<^sub>l_def
+    by (cases \<open>DECO_clause_l (get_trail_wl S')\<close>)
+      (auto simp: ran_m_mapsto_upd_notin all_lits_of_mm_add_mset blits_in_\<L>\<^sub>i\<^sub>n_def
+        in_\<L>\<^sub>a\<^sub>l\<^sub>l_atm_of_\<A>\<^sub>i\<^sub>n DECO_clause_l_DECO_clause[symmetric] Ball_def
+        in_all_lits_of_mm_ain_atms_of_iff all_conj_distrib
+        watched_by_alt_def get_unit_clauses_wl_alt_def
+        simp del: DECO_clause_l_DECO_clause)
+  ultimately show \<open>?eq \<Longrightarrow> literals_are_\<L>\<^sub>i\<^sub>n ?S'\<close>
+    unfolding literals_are_\<L>\<^sub>i\<^sub>n_def by blast
+qed
+
 
 lemma propagate_nonunit_and_add_wl_propagate_nonunit_and_add_wl:
   assumes
@@ -92,7 +163,8 @@ lemma propagate_nonunit_and_add_wl_propagate_nonunit_and_add_wl:
     (auto simp: ran_m_mapsto_upd_notin all_lits_of_mm_add_mset
     propagate_nonunit_and_add_wl_pre_def mset_take_mset_drop_mset'
     get_unit_clauses_wl_alt_def
-    intro!: is_\<L>\<^sub>a\<^sub>l\<^sub>l_add_all_lits_of_m)
+    intro!: is_\<L>\<^sub>a\<^sub>l\<^sub>l_add_all_lits_of_m
+   intro!: literals_are_\<L>\<^sub>i\<^sub>n_propagate_nonunit_and_add_wl)
 
 lemma negate_mode_bj_nonunit_wl_D_negate_mode_bj_nonunit_wl:
   fixes S S' :: \<open>nat twl_st_wl\<close>
@@ -108,14 +180,18 @@ proof -
       (find_decomp_target_wl (count_decided (get_trail_wl S')) S')\<close>
       (is \<open>_ \<le> \<Down> ?find_d _\<close>)
     using SS' unfolding find_decomp_target_wl_def
-    by (cases S') (auto simp: intro!: RES_refine)
-  have fresh: \<open>get_fresh_index (get_clauses_wl T)
-    \<le> \<Down> {(i, j). i = j \<and> i \<notin># dom_m (get_clauses_wl T)} (get_fresh_index (get_clauses_wl T'))\<close>
+    by (cases S') (auto simp: literals_are_\<L>\<^sub>i\<^sub>n_def blits_in_\<L>\<^sub>i\<^sub>n_def intro!: RES_refine)
+  have fresh: \<open>get_fresh_index_wl (get_clauses_wl T) (get_unit_clauses_wl T) (get_watched_wl T)
+    \<le> \<Down> {(i, j). i = j \<and> i \<notin># dom_m (get_clauses_wl T) \<and> i > 0 \<and>
+       (\<forall>L \<in># all_lits_of_mm (mset `# ran_mf (get_clauses_wl T) + get_unit_clauses_wl T) .
+          i \<notin> fst ` set (watched_by T L))}
+        (get_fresh_index_wl (get_clauses_wl T') (get_unit_clauses_wl T') (get_watched_wl T'))\<close>
     if \<open>(TK, TK') \<in> ?find_d\<close> and
       \<open>TK = (T, K)\<close> and
-      \<open>TK' = (T', K')\<close>
+      \<open>TK' =(T', K')\<close>
     for T T' K K' TK TK'
     using that by (auto simp: get_fresh_index_def equality_except_trail_wl_get_clauses_wl
+        get_fresh_index_wl_def watched_by_alt_def
       intro!: RES_refine)
   show ?thesis
     unfolding negate_mode_bj_nonunit_wl_D_def negate_mode_bj_nonunit_wl_def
@@ -144,8 +220,8 @@ fun restart_nonunit_and_add_wl_D
 where
   \<open>restart_nonunit_and_add_wl_D C i (M, N, D, NE, UE, Q, W) = do {
       ASSERT(restart_nonunit_and_add_wl_D_inv C i (M, N, D, NE, UE, Q, W));
-      let W = W(C!0 := W (C!0) @ [i]);
-      let W = W(C!1 := W (C!1) @ [i]);
+      let W = W(C!0 := W (C!0) @ [(i, C!1)]);
+      let W = W(C!1 := W (C!1) @ [(i, C!0)]);
       RETURN (M, fmupd i (C, True) N, None, NE, UE, {#}, W)
   }\<close>
 
@@ -157,7 +233,7 @@ where
     let C = DECO_clause_l (get_trail_wl S);
     i \<leftarrow> SPEC(\<lambda>i. i < count_decided (get_trail_wl S));
     (S, K) \<leftarrow> find_decomp_target_wl i S;
-    i \<leftarrow> get_fresh_index (get_clauses_wl S);
+    i \<leftarrow> get_fresh_index_wl (get_clauses_wl S) (get_unit_clauses_wl S) (get_watched_wl S);
     restart_nonunit_and_add_wl_D C i S
   })\<close>
 
@@ -195,7 +271,6 @@ lemma restart_nonunit_and_add_wl_D_restart_nonunit_and_add_wl:
 proof -
   have [simp]: \<open>i = i'\<close> and j: \<open>i' \<notin># dom_m (get_clauses_wl S)\<close>
     using ij by auto
-
   show ?thesis
     apply (cases T; cases T')
     apply (simp only: restart_nonunit_and_add_wl_D.simps
@@ -203,8 +278,9 @@ proof -
     apply refine_vcg
     subgoal using TK SS' ij unfolding restart_nonunit_and_add_wl_D_inv_def
       by auto
-    subgoal using TK SS' j unfolding restart_nonunit_and_add_wl_inv_def
-      by (fastforce simp: ran_m_mapsto_upd_notin all_lits_of_mm_add_mset
+    subgoal using TK SS' j literals_are_\<L>\<^sub>i\<^sub>n_propagate_nonunit_and_add_wl[of T S' i]
+      unfolding restart_nonunit_and_add_wl_inv_def
+      by (auto simp: ran_m_mapsto_upd_notin all_lits_of_mm_add_mset
        restart_nonunit_and_add_wl_D_inv_def mset_take_mset_drop_mset'
         restart_nonunit_and_add_wl_inv_def
         equality_except_trail_wl_get_clauses_wl[symmetric]
@@ -221,14 +297,17 @@ lemma negate_mode_restart_nonunit_wl_D_negate_mode_restart_nonunit_wl:
       \<Down> {(S, S''). (S, S'') \<in> Id \<and> literals_are_\<L>\<^sub>i\<^sub>n S}
        (negate_mode_restart_nonunit_wl S')\<close>
 proof -
-  have fresh: \<open>get_fresh_index (get_clauses_wl T)
-    \<le> \<Down> {(i, j). i = j \<and> i \<notin># dom_m (get_clauses_wl S)}
-       (get_fresh_index (get_clauses_wl T'))\<close>
+  have fresh: \<open>get_fresh_index_wl (get_clauses_wl T) (get_unit_clauses_wl T) (get_watched_wl T)
+    \<le> \<Down> {(i, j). i = j \<and> i \<notin># dom_m (get_clauses_wl T) \<and> i > 0 \<and>
+       (\<forall>L \<in># all_lits_of_mm (mset `# ran_mf (get_clauses_wl T) + get_unit_clauses_wl T) .
+          i \<notin> fst ` set (watched_by T L))}
+        (get_fresh_index_wl (get_clauses_wl T') (get_unit_clauses_wl T') (get_watched_wl T'))\<close>
     if \<open>(TK, TK') \<in> find_decomp_target_wl_D_ref S\<close> and
       \<open>TK = (T, K)\<close> and
       \<open>TK' =(T', K')\<close>
     for T T' K K' TK TK'
     using that by (auto simp: get_fresh_index_def equality_except_trail_wl_get_clauses_wl
+        get_fresh_index_wl_def watched_by_alt_def
       intro!: RES_refine)
   show ?thesis
     unfolding negate_mode_restart_nonunit_wl_def negate_mode_restart_nonunit_wl_D_def
@@ -241,6 +320,8 @@ proof -
     subgoal using SS' by auto
     subgoal using SS' by fast
     apply assumption+
+    subgoal for i ia x x' x1 x2 x1a x2a ib ic
+      using SS' by (cases S'; cases x1) auto
     done
 qed
 
